(rocq-checker) implement (vm/as)id tlbi

src/casemate-check-rocq/src/menhir_parser.mly
@@ -13,8 +13,6 @@
 %token READ
 %token DSB_ish DSB_ishst DSB_nsh
 %token ISB
-%token <string> TLBI_ALL
-%token <string> TLBI
 %token MSR
 %token SYSREG_VTTBR SYSREG_TTBR_EL2
 %token HINT
@@ -31,7 +29,7 @@
 
 trans:
     id= trans_id?
-    CPU COL cpu = NUM SCOL
+    CPU COL cpu = VAL
     data = trans_data
     AT
     src_loc = location
@@ -61,53 +59,53 @@ trans_data:
   | typ = write_types addr = VAL value = VAL { CMSD_TRANS_HW_MEM_WRITE {twd_mo = typ; twd_phys_addr = addr; twd_val = value} }
   | READ addr = VAL value = VAL { CMSD_TRANS_HW_MEM_READ { trd_phys_addr = addr; trd_val = value; } }
   | DSB_ish {CMSD_TRANS_HW_BARRIER (Barrier_DSB MBReqDomain_InnerShareable)}
-  | DSB_ishst {CMSD_TRANS_HW_BARRIER (Barrier_DSB MBReqDomain_FullSystem(* not sure *))}
+  | DSB_ishst {CMSD_TRANS_HW_BARRIER (Barrier_DSB MBReqDomain_InnerShareable)}
   | DSB_nsh {CMSD_TRANS_HW_BARRIER (Barrier_DSB MBReqDomain_OuterShareable)}
   | ISB { CMSD_TRANS_HW_BARRIER (Barrier_ISB ()) }
-  | tlbi = TLBI_ALL {
-    CMSD_TRANS_HW_TLBI (
-    let op, regime, shareability, level =
-      match tlbi with
-      | "TLBI_vmalls12e1" -> (TLBIOp_VMALLS12, Regime_EL10, Shareability_NSH, TLBILevel_Any)
-      | "TLBI_vmalle1is" -> (TLBIOp_VMALL, Regime_EL10, Shareability_ISH, TLBILevel_Any)
-      | "TLBI_vmalls12e1is" -> (TLBIOp_VMALLS12, Regime_EL10, Shareability_ISH, TLBILevel_Any)
-      | "TLBI_vmalle1" -> (TLBIOp_VMALL, Regime_EL10, Shareability_NSH, TLBILevel_Any)
-      | _ ->
-          Printf.eprintf "Unsupported TLBI operation %s\n" tlbi;
-          exit 1
-    in
-    {
-      tLBI_rec =
-        {
-          tLBIRecord_op = op;
-          tLBIRecord_regime = regime;
-          tLBIRecord_level = level;
-          tLBIRecord_address = Big_int_Z.zero_big_int;
-        };
-      tLBI_shareability = shareability;
-    })}
-  | tlbi = TLBI addr = VAL NUM {
-    CMSD_TRANS_HW_TLBI (
-      let op, regime, shareability, level =
-        match tlbi with
-        | "TLBI_alle1is" -> (TLBIOp_ALL, Regime_EL10, Shareability_ISH, TLBILevel_Any)
-        | "TLBI_vale2is" -> (TLBIOp_VA, Regime_EL2, Shareability_ISH, TLBILevel_Last)
-        | "TLBI_vae2is" -> (TLBIOp_VA, Regime_EL2, Shareability_ISH, TLBILevel_Any)
-        | "TLBI_ipas2e1is" -> (TLBIOp_IPAS2, Regime_EL10, Shareability_ISH, TLBILevel_Any)
-        | _ ->
-            Printf.eprintf "Unsupported TLBI operation %s\n" tlbi;
-            exit 1
-      in
-      {
-        tLBI_rec =
-          {
-            tLBIRecord_op = op;
-            tLBIRecord_regime = regime;
-            tLBIRecord_level = level;
-            tLBIRecord_address = addr;
-          };
-        tLBI_shareability = shareability;
-      })}
+  // | tlbi = TLBI_ALL {
+  //   CMSD_TRANS_HW_TLBI (
+  //   let op, regime, shareability, level =
+  //     match tlbi with
+  //     | "TLBI_vmalls12e1" -> (TLBIOp_VMALLS12, TLBI_REGIME_EL10, Shareability_NSH, TLBILevel_Any)
+  //     | "TLBI_vmalle1is" -> (TLBIOp_VMALL, TLBI_REGIME_EL10, Shareability_ISH, TLBILevel_Any)
+  //     | "TLBI_vmalls12e1is" -> (TLBIOp_VMALLS12, TLBI_REGIME_EL10, Shareability_ISH, TLBILevel_Any)
+  //     | "TLBI_vmalle1" -> (TLBIOp_VMALL, TLBI_REGIME_EL10, Shareability_NSH, TLBILevel_Any)
+  //     | _ ->
+  //         Printf.eprintf "Unsupported TLBI operation %s\n" tlbi;
+  //         exit 1
+  //   in
+  //   {
+  //     tLBI_rec =
+  //       {
+  //         tLBIRecord_op = op;
+  //         tLBIRecord_regime = regime;
+  //         tLBIRecord_level = level;
+  //         tLBIRecord_address = Big_int_Z.zero_big_int;
+  //       };
+  //     tLBI_shareability = shareability;
+  //   })}
+  // | tlbi = TLBI addr = VAL NUM {
+  //   CMSD_TRANS_HW_TLBI (
+  //     let op, regime, shareability, level =
+  //       match tlbi with
+  //       | "TLBI_alle1is" -> (TLBIOp_ALL, TLBI_REGIME_EL10, Shareability_ISH, TLBILevel_Any)
+  //       | "TLBI_vale2is" -> (TLBIOp_VA, TLBI_REGIME_EL2, Shareability_ISH, TLBILevel_Last)
+  //       | "TLBI_vae2is" -> (TLBIOp_VA, TLBI_REGIME_EL2, Shareability_ISH, TLBILevel_Any)
+  //       | "TLBI_ipas2e1is" -> (TLBIOp_IPAS2, TLBI_REGIME_EL10, Shareability_ISH, TLBILevel_Any)
+  //       | _ ->
+  //           Printf.eprintf "Unsupported TLBI operation %s\n" tlbi;
+  //           exit 1
+  //     in
+  //     {
+  //       tLBI_rec =
+  //         {
+  //           tLBIRecord_op = op;
+  //           tLBIRecord_regime = regime;
+  //           tLBIRecord_level = level;
+  //           tLBIRecord_address = addr;
+  //         };
+  //       tLBI_shareability = shareability;
+  //     })}
   | MSR reg = sysreg addr = VAL { CMSD_TRANS_HW_MSR {tmd_sysreg = reg; tmd_val = addr; } }
   | HINT kind = hint_type loc = VAL value = VAL { CMSD_TRANS_HINT {thd_hint_kind = kind; thd_location = loc; thd_value = value} }
   | HINT kind = hint_type loc = VAL { CMSD_TRANS_HINT {thd_hint_kind = kind; thd_location = loc; thd_value = Big_int_Z.big_int_of_int 0} }
@@ -119,7 +117,7 @@ trans_data:
 write_types:
   | W {WMO_plain}
   | Wrel {WMO_release}
-  | Wpage {WMO_page}
+  // | Wpage {WMO_page}
 
 sysreg:
   | SYSREG_VTTBR {SYSREG_VTTBR}
