src/casemate-check-rocq/theories/transition.v
@@ -3,11 +3,22 @@ Require Import model.
 Require Import pgtable.
 
 (* Inductive SecurityState := SS_NonSecure | SS_Root | SS_Realm | SS_Secure. *)
-Inductive Regime := Regime_EL3 | Regime_EL30 | Regime_EL2 | Regime_EL20 | Regime_EL10.
-Inductive Shareability := Shareability_NSH | Shareability_ISH | Shareability_OSH.
+Inductive Regime := 
+  | TLBI_REGIME_EL3
+  | TLBI_REGIME_EL30
+  | TLBI_REGIME_EL2
+  | TLBI_REGIME_EL20
+  | TLBI_REGIME_EL10
+.
+
+Inductive Shareability := 
+  | Shareability_NSH
+  | Shareability_ISH 
+  | Shareability_OSH
+.
 
 (** TLBI *)
-Inductive TLBIOp :=
+(* Inductive TLBIOp :=
   | TLBIOp_DALL
   | TLBIOp_DASID
   | TLBIOp_DVA
@@ -26,11 +37,11 @@ Inductive TLBIOp :=
   | TLBIOp_RVA
   | TLBIOp_RPA
   | TLBIOp_PAALL
-.
+. *)
 
 Inductive TLBILevel := TLBILevel_Any | TLBILevel_Last.
 
-Record TLBIRecord  := {
+(* Record TLBIRecord  := {
   TLBIRecord_op : TLBIOp;
   (* TLBIRecord_from_aarch64 : bool; *)
   (* TLBIRecord_security : SecurityState; *)
@@ -49,7 +60,7 @@ Record TLBIRecord  := {
 Record TLBI := {
   TLBI_rec : TLBIRecord;
   TLBI_shareability : Shareability;
-}.
+}. *)
 
 Inductive TLBI_stage_kind :=
   | TLBI_OP_stage1
@@ -59,13 +70,15 @@ Inductive TLBI_stage_kind :=
 
 Record TLBI_op_by_addr_data := {
   TOBAD_page : phys_addr_t;
-  TOBAD_last_level_only : TLBILevel;
+  TOBAD_level_hint : option u64;
+  TOBAD_last_level_only : bool;
+  TOBAD_asid : option addr_id_t;
 }.
 
 Inductive TLBI_method :=
   | TLBI_by_addr_space : phys_addr_t -> TLBI_method
   | TLBI_by_input_addr : TLBI_op_by_addr_data -> TLBI_method
-  | TLBI_by_addr_all
+  | TLBI_by_all
 .
 
 Record TLBI_intermediate := {
@@ -75,53 +88,121 @@ Record TLBI_intermediate := {
   TI_method : TLBI_method;
 }.
 
-Definition decode_tlbi_stage (td : TLBI) : option TLBI_stage_kind :=
-  match td.(TLBI_rec).(TLBIRecord_op) with
-  | TLBIOp_VA 
-  | TLBIOp_VMALL => Some TLBI_OP_stage1
-  | TLBIOp_IPAS2 => Some TLBI_OP_stage2
-  | TLBIOp_VMALLS12 
-  | TLBIOp_ALL => Some TLBI_OP_both_stages
-  | _ => None
-  end
+Inductive tlbi_kind :=
+  | TLBI_vmalls12e1
+	| TLBI_vmalls12e1is
+	| TLBI_vmalle1is
+	| TLBI_alle1is
+  | TLBI_vae2
+	| TLBI_vmalle1
+	| TLBI_vale2is
+	| TLBI_vae2is
+	| TLBI_ipas2e1is
 .
 
-Definition decode_tlbi_shootdown (td : TLBI) : option bool :=
-  match td.(TLBI_shareability) with
-  | Shareability_ISH => Some true
-  | _ => Some true
-  end
-.
+Record trans_tlbi_data := {
+  ttd_tlbi_kind : tlbi_kind;
+  ttd_value : u64
+}.
 
-Definition decode_tlbi_method (td : TLBI) : option TLBI_method :=
-  match td.(TLBI_rec).(TLBIRecord_op) with
-  | TLBIOp_VMALLS12 | TLBIOp_VMALL =>
-    Some TLBI_by_addr_all
-  | TLBIOp_VA | TLBIOp_IPAS2 =>
-    Some (TLBI_by_input_addr
-          {| TOBAD_page := td.(TLBI_rec).(TLBIRecord_address);
-            TOBAD_last_level_only := td.(TLBI_rec).(TLBIRecord_level); |})
-  | TLBIOp_ALL => Some TLBI_by_addr_all
-  | _ => None
-  end
-.
+Definition decode_tlbi_stage (td : trans_tlbi_data) : TLBI_stage_kind :=
+  match td.(ttd_tlbi_kind) with
+  | TLBI_vmalls12e1 => TLBI_OP_both_stages
+	| TLBI_vmalls12e1is => TLBI_OP_both_stages
+	| TLBI_vmalle1is => TLBI_OP_stage1
+	| TLBI_alle1is => TLBI_OP_stage1
+  | TLBI_vae2 => TLBI_OP_stage1
+	| TLBI_vmalle1 => TLBI_OP_stage1
+	| TLBI_vale2is => TLBI_OP_stage1
+	| TLBI_vae2is => TLBI_OP_stage1
+	| TLBI_ipas2e1is => TLBI_OP_stage2
+  end.
 
-Definition decode_tlbi (td : TLBI) : option TLBI_intermediate :=
+Definition decode_tlbi_regime (td : trans_tlbi_data) : Regime :=
+  match td.(ttd_tlbi_kind) with
+  | TLBI_vmalle1is
+	| TLBI_vmalle1
+	| TLBI_ipas2e1is
+	| TLBI_vmalls12e1
+	| TLBI_vmalls12e1is
+	| TLBI_alle1is => TLBI_REGIME_EL10
+  | TLBI_vale2is
+	| TLBI_vae2is
+  | TLBI_vae2 => TLBI_REGIME_EL2
+  end.
+
+Definition decode_tlbi_shootdown (td : trans_tlbi_data) : bool :=
+  match td.(ttd_tlbi_kind) with
+  | TLBI_vmalls12e1 => false
+	| TLBI_vmalls12e1is => true
+	| TLBI_vmalle1is => true
+	| TLBI_alle1is => true
+	| TLBI_vmalle1 => false
+  | TLBI_vae2 => false (* TODO: missing kind in C *)
+	| TLBI_vale2is => true
+	| TLBI_vae2is => true
+	| TLBI_ipas2e1is => true
+  end.
+
+Definition decoded_tlbi_has_asid (td : trans_tlbi_data) : option addr_id_t :=
+  match td.(ttd_tlbi_kind) with
+  | TLBI_vale2is
+	| TLBI_vae2is => Some (AID (bv_and_64 td.(ttd_value) TLBI_ASID_MASK))
+  | TLBI_vmalls12e1 => None
+	| TLBI_vmalls12e1is => None
+	| TLBI_vmalle1is => None
+	| TLBI_alle1is => None
+	| TLBI_vmalle1 => None
+  | TLBI_vae2 => None
+	| TLBI_ipas2e1is => None
+  end.
+
+Definition decode_tlbi_by_addr (td : trans_tlbi_data) : TLBI_op_by_addr_data :=
+  let page := bv_and_64 td.(ttd_value) TLBI_PAGE_MASK in
+  let last_level_only := 
+    match td.(ttd_tlbi_kind) with
+    | TLBI_vale2is => true
+    | _ => false
+    end in
+  let level := bv_and_64 td.(ttd_value) TLBI_TTL_MASK in
+  let level_hint := 
+    if (level b<? b4) then None 
+    else Some (bv_and_64 level b3) in
+
+  {|
+    TOBAD_page := PA page;
+    TOBAD_last_level_only := last_level_only;
+    TOBAD_level_hint := level_hint;
+    TOBAD_asid := decoded_tlbi_has_asid td;
+  |}.
+
+Definition decode_tlbi_by_space_id (td : trans_tlbi_data) : phys_addr_t := PA b0.
+
+Definition decode_tlbi_method (td : trans_tlbi_data) : TLBI_method :=
+  match td.(ttd_tlbi_kind) with
+  | TLBI_vmalls12e1
+	| TLBI_vmalls12e1is
+	| TLBI_vmalle1is
+  | TLBI_vmalle1 => TLBI_by_addr_space (decode_tlbi_by_space_id td)
+  | TLBI_vale2is
+  | TLBI_vae2
+  | TLBI_vae2is
+  | TLBI_ipas2e1is => TLBI_by_input_addr (decode_tlbi_by_addr td)
+	| TLBI_alle1is => TLBI_by_all
+  end.
+
+Definition decode_tlbi (td : trans_tlbi_data) : TLBI_intermediate :=
   let stage := decode_tlbi_stage td in
+  let regime := decode_tlbi_regime td in
   let shootdown := decode_tlbi_shootdown td in
   let method := decode_tlbi_method td in
-  match stage, shootdown, method with
-  | Some stage, Some shootdown, Some method =>
-    Some
-    {|
-      TI_stage := stage;
-      TI_regime := td.(TLBI_rec).(TLBIRecord_regime);
-      TI_shootdown := shootdown;
-      TI_method := method;
-    |}
-  | _, _, _ => None
-  end
-.
+  
+  {|
+    TI_stage := stage;
+    TI_regime := regime;
+    TI_shootdown := shootdown;
+    TI_method := method;
+  |}.
 
 
 (** Barrier *)
@@ -157,7 +238,6 @@ Inductive Barrier :=
 (* All those transitions will go in favor of ARM ISA description (except for hints) *)
 Inductive write_memory_order :=
   | WMO_plain
-  | WMO_page
   | WMO_release
 .
 
@@ -225,7 +305,7 @@ Inductive casemate_model_step_data :=
   | CMSD_TRANS_HW_MEM_WRITE (write_data : trans_write_data)
   | CMSD_TRANS_HW_MEM_READ (read_data : trans_read_data)
   | CMSD_TRANS_HW_BARRIER (dsb_data : Barrier)
-  | CMSD_TRANS_HW_TLBI (tlbi_data : TLBI)
+  | CMSD_TRANS_HW_TLBI (tlbi_data : trans_tlbi_data)
   | CMSD_TRANS_HW_MSR (msr_data : trans_msr_data)
   (* ABS_step *)
   | CMSD_TRANS_ABS_MEM_INIT (init_data : trans_init_data)
@@ -253,7 +333,7 @@ Definition clean_reachable_cb (ctx : pgtable_traverse_context) : casemate_model_
     match location.(sl_pte) with
     | None => Mreturn ctx.(ptc_state)
     | Some descriptor =>
-      match descriptor.(ged_state) with
+      match descriptor.(eed_state) with
       | SPS_STATE_PTE_INVALID_UNCLEAN _ =>
         Merror (CME_unclean_child ctx.(ptc_addr))
       | _ => Mreturn ctx.(ptc_state)
@@ -263,41 +343,40 @@ Definition clean_reachable_cb (ctx : pgtable_traverse_context) : casemate_model_
 
 Definition clean_reachable
   (map : table_data_t)
-  (descriptor : ghost_exploded_descriptor)
+  (descriptor : entry_exploded_descriptor)
   (cm : casemate_model_state):
   casemate_model_result :=
   traverse_pgt_from
-    descriptor.(ged_owner)
+    descriptor.(eed_owner)
     map.(next_level_table_addr)
-    descriptor.(ged_ia_region).(range_start)
-    (next_level descriptor.(ged_level))
-    descriptor.(ged_stage)
+    descriptor.(eed_ia_region).(range_start)
+    (next_level descriptor.(eed_level))
+    descriptor.(eed_stage)
     clean_reachable_cb
-    cm
-.
+    cm.
 
 Definition step_write_table_mark_children
   (tid : thread_identifier)
   (wmo : write_memory_order)
   (loc : sm_location)
   (val : u64)
-  (descriptor : ghost_exploded_descriptor)
+  (descriptor : entry_exploded_descriptor)
   (visitor_cb : pgtable_traverse_context -> casemate_model_result)
   (cm : casemate_model_state) :
   casemate_model_result :=
   if is_desc_valid val then
     (* Tests if the page table is well formed *)
-    match descriptor.(ged_pte_kind) with
+    match descriptor.(eed_pte_kind) with
     | PTER_PTE_KIND_TABLE map =>
       let st := clean_reachable map descriptor cm in
       let st := Mlog
         (Log "BBM: invalid clean->valid"%string (phys_addr_val loc.(sl_phys_addr))) st in
       Mupdate_state (traverse_pgt_from
-                        descriptor.(ged_owner)
+                        descriptor.(eed_owner)
                         map.(next_level_table_addr)
-                        descriptor.(ged_ia_region).(range_start)
-                        (next_level descriptor.(ged_level))
-                        descriptor.(ged_stage)
+                        descriptor.(eed_ia_region).(range_start)
+                        (next_level descriptor.(eed_level))
+                        descriptor.(eed_stage)
                         visitor_cb) st
     | _ => Mlog
           (Log "BBM: invalid clean->valid"%string (phys_addr_val loc.(sl_phys_addr))) (Mreturn cm)
@@ -320,15 +399,14 @@ Definition step_write_on_invalid
     | Some descriptor =>
       let descriptor := deconstruct_pte
           tid
-          descriptor.(ged_ia_region).(range_start)
-          val descriptor.(ged_level)
-          descriptor.(ged_owner)
-          descriptor.(ged_stage) in
+          descriptor.(eed_ia_region).(range_start)
+          val descriptor.(eed_level)
+          descriptor.(eed_owner)
+          descriptor.(eed_stage) in
       let new_loc := loc <| sl_val := val |> <| sl_pte := Some descriptor |> in
-      let new_cm := cm <| cm_memory := <[ loc.(sl_phys_addr) := new_loc ]> cm.(cm_memory) |> in
+      let new_cm := cm <| cms_memory := <[ loc.(sl_phys_addr) := new_loc ]> cm.(cms_memory) |> in
       step_write_table_mark_children tid wmo loc val descriptor (mark_cb tid) new_cm
-    end
-.
+    end.
 
 Definition step_write_on_invalid_unclean
   (tid : thread_identifier)
@@ -341,8 +419,7 @@ Definition step_write_on_invalid_unclean
   if is_desc_valid val then
     (Merror (CME_bbm_violation VT_valid_on_invalid_unclean loc.(sl_phys_addr)))
   else
-    Mreturn (cm <|cm_memory := <[loc.(sl_phys_addr) := loc <|sl_val := val|> ]> cm.(cm_memory) |>)
-.
+    Mreturn (cm <|cms_memory := <[loc.(sl_phys_addr) := loc <|sl_val := val|> ]> cm.(cms_memory) |>).
 
 Definition is_only_update_to_sw_bit (old new : u64) : bool :=
   (bv_and_64 old NOT_PTE_FIELD_UPPER_ATTRS_SW_MASK) b=? (bv_and_64 new NOT_PTE_FIELD_UPPER_ATTRS_SW_MASK)
@@ -356,8 +433,8 @@ Definition require_bbm
   match loc.(sl_pte) with
   | None => None (* PTE cannot be valid if it is not a PTE *)
   | Some old_descriptor =>
-    let new_descriptor := deconstruct_pte tid old_descriptor.(ged_ia_region).(range_start) val old_descriptor.(ged_level) old_descriptor.(ged_owner) old_descriptor.(ged_stage) in
-    match old_descriptor.(ged_pte_kind), new_descriptor.(ged_pte_kind) with
+    let new_descriptor := deconstruct_pte tid old_descriptor.(eed_ia_region).(range_start) val old_descriptor.(eed_level) old_descriptor.(eed_owner) old_descriptor.(eed_stage) in
+    match old_descriptor.(eed_pte_kind), new_descriptor.(eed_pte_kind) with
     | PTER_PTE_KIND_INVALID, _ | _, PTER_PTE_KIND_INVALID => Some false
     | PTER_PTE_KIND_TABLE _, _ | _, PTER_PTE_KIND_TABLE _ => Some true
     | PTER_PTE_KIND_MAP r1, PTER_PTE_KIND_MAP r2 =>
@@ -366,8 +443,7 @@ Definition require_bbm
       else
         Some (negb (is_only_update_to_sw_bit loc.(sl_val) val))
     end
-  end
-.
+  end.
 
 Definition step_write_valid_on_valid
   (tid : thread_identifier)
@@ -384,15 +460,14 @@ Definition step_write_valid_on_valid
       | None => (* This does not make sense because function is called on a pgt *)
         Merror (CME_internal_error IET_unexpected_none)
       | Some pte =>
-        let new_pte := deconstruct_pte tid pte.(ged_ia_region).(range_start) val pte.(ged_level) pte.(ged_owner) pte.(ged_stage) in
+        let new_pte := deconstruct_pte tid pte.(eed_ia_region).(range_start) val pte.(eed_level) pte.(eed_owner) pte.(eed_stage) in
         let loc := loc <| sl_val := val |> <| sl_pte := Some new_pte |> in
         Mreturn (insert_location loc cm)
       end
   | Some true =>
     (* Changing the descriptor is illegal *)
     Merror (CME_bbm_violation VT_valid_on_valid loc.(sl_phys_addr))
-  end
-.
+  end.
 
 Definition step_write_invalid_on_valid
   (tid : thread_identifier)
@@ -407,10 +482,10 @@ Definition step_write_invalid_on_valid
   | None => (* This does not make sense because function is called on a pgt *)
       Merror (CME_internal_error IET_unexpected_none)
   | Some descriptor =>
-    let new_desc := descriptor <| ged_state := (SPS_STATE_PTE_INVALID_UNCLEAN {| ai_invalidator_tid := tid; ai_old_valid_desc :=  old; ai_lis := LIS_unguarded; |}) |> in
-    let cm := (cm <| cm_memory := (<[ loc.(sl_phys_addr) := loc <|sl_pte := Some (new_desc)|> <| sl_val := val |> ]> cm.(cm_memory))|> ) in
+    let new_desc := descriptor <| eed_state := (SPS_STATE_PTE_INVALID_UNCLEAN {| ai_invalidator_tid := tid; ai_old_valid_desc :=  old; ai_lis := LIS_unguarded; |}) |> in
+    let cm := (cm <| cms_memory := (<[ loc.(sl_phys_addr) := loc <|sl_pte := Some (new_desc)|> <| sl_val := val |> ]> cm.(cms_memory))|> ) in
     Mlog (Log "BBM: valid->invalid_unclean"%string (phys_addr_val loc.(sl_phys_addr)))
-    match descriptor.(ged_pte_kind) with
+    match descriptor.(eed_pte_kind) with
     | PTER_PTE_KIND_TABLE map =>
       let res := clean_reachable map descriptor cm in
       let res := Mlog (Log "invalidating a table descriptor"%string (phys_addr_val loc.(sl_phys_addr))) res in
@@ -418,8 +493,7 @@ Definition step_write_invalid_on_valid
       Mupdate_state (step_write_table_mark_children tid wmo loc val descriptor (mark_not_writable_cb tid)) res
     | _ => Mreturn cm
     end
-  end
-.
+  end.
 
 Definition step_write_on_valid
   (tid : thread_identifier)
@@ -441,35 +515,35 @@ Definition is_valid_state (st: sm_pte_state) : bool :=
   end
 .
 
-Definition drop_write_authorization_of_lock
+Definition drop_write_authorization
   (cpu : thread_identifier)
   (addr : phys_addr_t)
   (wmo : write_memory_order)
   (descriptor : u64)
-  (pte : ghost_exploded_descriptor)
+  (pte : entry_exploded_descriptor)
   (cm : casemate_model_state) : casemate_model_result :=
-  match get_lock_of_owner pte.(ged_owner) cm with
-  | None => Mreturn cm
-  | Some addr_lock =>
-    match lookup addr_lock cm.(cm_lock_state) with
+  match get_lock_of_owner pte.(eed_owner) cm with
+  | None => Merror CME_owner_not_associated
+  | Some lock_addr =>
+    match lookup lock_addr cm.(cms_lock_state) with
     | Some {| ls_tid := lock_owner; ls_write_authorization := auth |} =>
       if bool_decide (lock_owner = cpu) then
         match wmo with
-        | WMO_page | WMO_plain => (* check that the write is authorized, and then drop the authorization *)
+        | WMO_plain => (* check that the write is authorized, and then drop the authorization *)
           match auth with
           | WA_AUTHORIZED => 
             let new_lock_state := {| ls_tid := lock_owner; ls_write_authorization := WA_UNAUTHORIZED |} in
-            Mreturn (cm <| cm_lock_state := insert addr_lock new_lock_state cm.(cm_lock_state)|>)
+            Mreturn (cm <| cms_lock_state := insert lock_addr new_lock_state cm.(cms_lock_state)|>)
           | WA_UNAUTHORIZED =>
-            if (is_desc_valid descriptor) || is_valid_state pte.(ged_state) then
+            if (is_desc_valid descriptor) || is_valid_state pte.(eed_state) then
               Merror (CME_write_without_authorization addr)
             else
               let new_lock_state := {| ls_tid := lock_owner; ls_write_authorization := WA_UNAUTHORIZED |} in
-              Mreturn (cm <| cm_lock_state := insert addr_lock new_lock_state cm.(cm_lock_state)|>)
+              Mreturn (cm <| cms_lock_state := insert lock_addr new_lock_state cm.(cms_lock_state)|>)
           end
         | WMO_release => (* drop the authorization *)
           let new_lock_state := {| ls_tid := lock_owner; ls_write_authorization := WA_UNAUTHORIZED |} in
-          Mreturn (cm <| cm_lock_state := insert addr_lock new_lock_state cm.(cm_lock_state)|>)
+          Mreturn (cm <| cms_lock_state := insert lock_addr new_lock_state cm.(cms_lock_state)|>)
         end
       else
         Merror (CME_transition_without_lock addr)
@@ -477,7 +551,7 @@ Definition drop_write_authorization_of_lock
     end
   end.
 
-Definition drop_write_authorization
+Definition check_write_authorized
   (tid : thread_identifier)
   (wd : trans_write_data)
   (cm : casemate_model_state) :
@@ -494,37 +568,41 @@ Definition drop_write_authorization
         match location.(sl_pte) with
         | None => Mreturn cm
         | Some pte =>
-          if is_loc_thread_owned tid location cm then
-            Mreturn cm
-          else
-            drop_write_authorization_of_lock tid addr wmo val pte cm
+          match location.(sl_thread_owner) with
+          | Some thread_owner =>
+            if bool_decide (thread_owner = tid) then
+              Mreturn cm
+            else
+              Merror (CME_owned_pte_accessed_by_other_thread addr)
+          | None => drop_write_authorization tid addr wmo val pte cm
+          end
         end
-    end
-.
+    end.
 
-Definition step_write_aux
+Definition step_write
   (tid : thread_identifier)
   (wd : trans_write_data)
-  (cm : casemate_model_state) : casemate_model_result :=
-  let wmo := wd.(twd_mo) in
+  (cm : casemate_model_state) : 
+  casemate_model_result :=
+  let mo := wd.(twd_mo) in
   let val := wd.(twd_val) in
   let addr := wd.(twd_phys_addr) in
   if negb ((bv_and_64 (phys_addr_val addr) b7) b=? b0)
     then Merror CME_unaligned_write else
-  let new_st := drop_write_authorization tid wd cm in
+  let new_st := check_write_authorized tid wd cm in
   let write_update s :=
     match s !! addr with
     | Some (loc) =>
       match loc.(sl_pte) with
       | Some desc =>
         (* If we write to a page table, depending on its state, we update them  *)
-        match desc.(ged_state) with
+        match desc.(eed_state) with
         | SPS_STATE_PTE_VALID av =>
-            (step_write_on_valid tid wmo loc val s)
+            (step_write_on_valid tid mo loc val s)
         | SPS_STATE_PTE_INVALID_CLEAN av =>
-            (step_write_on_invalid tid wmo loc val s)
+            (step_write_on_invalid tid mo loc val s)
         | SPS_STATE_PTE_INVALID_UNCLEAN av =>
-            (step_write_on_invalid_unclean tid wmo loc val s)
+            (step_write_on_invalid_unclean tid mo loc val s)
         | SPS_STATE_PTE_NOT_WRITABLE =>
             (Merror (CME_write_on_not_writable addr))
         end
@@ -534,25 +612,24 @@ Definition step_write_aux
           cmr_log := nil;
           cmr_data :=
             Ok _ _ (
-              s <| cm_memory := <[ addr := new_loc ]> s.(cm_memory) |>
+              s <| cms_memory := <[ addr := new_loc ]> s.(cms_memory) |>
             );
         |}
       end
     | None =>
       (* If the location has not been written to, it is not a pgt, just save its value *)
-        let new_st := s <| cm_memory :=
+        let new_st := s <| cms_memory :=
             <[ addr := {|
                 sl_phys_addr := addr;
                 sl_val := val;
                 sl_pte := None;
                 sl_thread_owner := None;
               |}
-            ]> s.(cm_memory) |> in
+            ]> s.(cms_memory) |> in
                 Mreturn new_st
-          end
+    end
   in
-  Mupdate_state write_update new_st
-.
+  Mupdate_state write_update new_st.
 
 Function step_write_page
   (tid : thread_identifier)
@@ -571,18 +648,9 @@ Function step_write_page
         twd_val := wd.(twd_val);
       |}
     in
-    let res := Mupdate_state (step_write_aux tid sub_wd) res in
+    let res := Mupdate_state (step_write tid sub_wd) res in
     step_write_page tid wd res (offs - 1).
 Proof. lia. Qed.
-
-Definition step_write
-  (tid : thread_identifier)
-  (wd : trans_write_data)
-  (cm : casemate_model_state) : casemate_model_result :=
-  match wd.(twd_mo) with
-  | WMO_plain | WMO_release => step_write_aux tid wd cm
-  | WMO_page => step_write_page tid wd (Mreturn cm) z512
-  end.
 
 (** Mem init *)
 
@@ -590,10 +658,10 @@ Definition step_init_aux
   (addr : phys_addr_t)
   (st : casemate_model_result) :
   casemate_model_result :=
-  let update s := {| cmr_log := nil; cmr_data := Ok _ _ (s <| cm_initialised := <[ addr := () ]> s.(cm_initialised) |>) |} in
+  let update s := {| cmr_log := nil; cmr_data := Ok _ _ (s <| cms_initialised := <[ addr := () ]> s.(cms_initialised) |>) |} in
   Mupdate_state update st.
 
-Definition _step_init_step_size := PA (bv_shiftl_64 b1 (bv64.BV64 3)).
+Definition _step_init_step_size := PA (bv_shiftl_64 b1 b3).
 
 Fixpoint step_init_all
   (addr : phys_addr_t)
@@ -642,10 +710,10 @@ Definition step_read
         let new_loc := loc <| sl_val := rd.(trd_val) |> in
         {| cmr_log :=
             [Inconsistent_read loc.(sl_val) rd.(trd_val) rd.(trd_phys_addr)];
-           cmr_data := (Ok _ _ (cm <| cm_memory := <[rd.(trd_phys_addr) := new_loc ]> cm.(cm_memory) |>)) |}
+           cmr_data := (Ok _ _ (cm <| cms_memory := <[rd.(trd_phys_addr) := new_loc ]> cm.(cms_memory) |>)) |}
   | None =>
       let loc := {| sl_phys_addr := rd.(trd_phys_addr); sl_val := rd.(trd_val); sl_pte := None; sl_thread_owner := Some tid |} in
-      let st := cm <| cm_memory := <[ rd.(trd_phys_addr) := loc ]> cm.(cm_memory) |> in
+      let st := cm <| cms_memory := <[ rd.(trd_phys_addr) := loc ]> cm.(cms_memory) |> in
       {| cmr_log :=
           [Warning_read_write_non_allocd loc.(sl_phys_addr)];
          cmr_data := Ok _ _ st
@@ -664,19 +732,19 @@ Definition dsb_invalid_unclean_unmark_children
   let desc := (* This uses the old descriptor to rebuild a fresh old descriptor *)
     deconstruct_pte cpu_id ptc.(ptc_partial_ia) lis.(ai_old_valid_desc) ptc.(ptc_level) ptc.(ptc_root) ptc.(ptc_stage)
   in
-  match desc.(ged_pte_kind) with
+  match desc.(eed_pte_kind) with
   | PTER_PTE_KIND_TABLE map =>
     (* The children are clean, and not writable, otherwise, it would catch fire *)
-    traverse_pgt_from desc.(ged_owner) map.(next_level_table_addr) desc.(ged_ia_region).(range_start) (next_level desc.(ged_level)) desc.(ged_stage) (unmark_cb cpu_id) st
+    traverse_pgt_from desc.(eed_owner) map.(next_level_table_addr) desc.(eed_ia_region).(range_start) (next_level desc.(eed_level)) desc.(eed_stage) (unmark_cb cpu_id) st
   | _ => {| cmr_log  := nil; cmr_data := Ok _ _ st |}
   end.
 
 
 Definition new_pte_after_dsb
   (cpu_id : thread_identifier)
-  (pte : ghost_exploded_descriptor)
-  (kind : DxB) : ghost_exploded_descriptor :=
-  match pte.(ged_state) with
+  (pte : entry_exploded_descriptor)
+  (kind : DxB) : entry_exploded_descriptor :=
+  match pte.(eed_state) with
   | SPS_STATE_PTE_INVALID_UNCLEAN sst =>
     (* DSB has an effect on invalid unclean state only *)
     if negb (bool_decide (sst.(ai_invalidator_tid) = cpu_id)) then
@@ -685,19 +753,19 @@ Definition new_pte_after_dsb
       (* Otherwise, update the state invalid unclean sub-automaton *)
       match sst.(ai_lis) with
       | LIS_unguarded =>
-        pte <|ged_state := SPS_STATE_PTE_INVALID_UNCLEAN (sst <| ai_lis := LIS_dsbed |>) |>
+        pte <|eed_state := SPS_STATE_PTE_INVALID_UNCLEAN (sst <| ai_lis := LIS_dsbed |>) |>
       | LIS_dsbed => pte
       | LIS_dsb_tlbied =>
         match kind.(DxB_domain) with
         | MBReqDomain_InnerShareable | MBReqDomain_FullSystem =>
-          pte <| ged_state := SPS_STATE_PTE_INVALID_CLEAN {| aic_invalidator_tid := sst.(ai_invalidator_tid) |} |>
-              <| ged_pte_kind := PTER_PTE_KIND_INVALID |>
+          pte <| eed_state := SPS_STATE_PTE_INVALID_CLEAN {| aic_invalidator_tid := sst.(ai_invalidator_tid) |} |>
+              <| eed_pte_kind := PTER_PTE_KIND_INVALID |>
         | _ => pte
         end
       | LIS_dsb_tlbi_ipa =>
           match kind.(DxB_domain) with
           | MBReqDomain_InnerShareable | MBReqDomain_FullSystem =>
-            pte <|ged_state := SPS_STATE_PTE_INVALID_UNCLEAN (sst <|ai_lis := LIS_dsb_tlbi_ipa_dsb |>) |>
+            pte <|eed_state := SPS_STATE_PTE_INVALID_UNCLEAN (sst <|ai_lis := LIS_dsb_tlbi_ipa_dsb |>) |>
           | _ => pte
           end
       | _ => pte
@@ -720,9 +788,9 @@ Definition dsb_visitor
       let new_pte := new_pte_after_dsb cpu_id pte kind in
       (* then update state and return *)
       let new_loc := (location <| sl_pte := Some new_pte |>) in
-      let new_state := ctx.(ptc_state) <| cm_memory := <[ location.(sl_phys_addr) := new_loc ]> ctx.(ptc_state).(cm_memory) |> in
+      let new_state := ctx.(ptc_state) <| cms_memory := <[ location.(sl_phys_addr) := new_loc ]> ctx.(ptc_state).(cms_memory) |> in
       let log :=
-        match pte.(ged_state), new_pte.(ged_state) with
+        match pte.(eed_state), new_pte.(eed_state) with
         | SPS_STATE_PTE_INVALID_UNCLEAN _ , SPS_STATE_PTE_INVALID_CLEAN _ =>
           Some (Log "BBM: invalid_unclean->invalid_clean"%string (phys_addr_val location.(sl_phys_addr)))
         | SPS_STATE_PTE_INVALID_UNCLEAN {| ai_lis := LIS_unguarded|} , SPS_STATE_PTE_INVALID_UNCLEAN {| ai_lis := _|} =>
@@ -733,7 +801,7 @@ Definition dsb_visitor
         end
       in
       let new_state :=
-        match pte.(ged_state), new_pte.(ged_state) with
+        match pte.(eed_state), new_pte.(eed_state) with
         | SPS_STATE_PTE_INVALID_UNCLEAN lis , SPS_STATE_PTE_INVALID_CLEAN _ =>
           dsb_invalid_unclean_unmark_children cpu_id new_loc lis
               (ctx <| ptc_state := new_state |> <|ptc_loc := Some new_loc|>)
@@ -755,16 +823,16 @@ Fixpoint reset_write_authorizations_aux
   match roots with
   | [] => cm
   | {| r_baddr := baddr; r_id := _; r_refcount := _ |} :: q =>
-    match lookup (phys_addr_val (root_val baddr)) cm.(cm_lock_addr) with
+    match lookup (phys_addr_val (root_val baddr)) cm.(cms_lock_addr) with
     | Some lock_addr =>
       let new_st :=
-        match lookup lock_addr cm.(cm_lock_state) with
+        match lookup lock_addr cm.(cms_lock_state) with
         | None => cm
         | Some {| ls_tid := thread; ls_write_authorization := _ |} =>
           if bool_decide (thread = tid) then
             let new_lock_state := {| ls_tid := tid; ls_write_authorization := WA_AUTHORIZED |} in
-            (cm <| cm_lock_state :=
-                insert lock_addr new_lock_state cm.(cm_lock_state) |>)
+            (cm <| cms_lock_state :=
+                insert lock_addr new_lock_state cm.(cms_lock_state) |>)
           else
             cm
         end
@@ -779,8 +847,8 @@ Definition reset_write_authorizations
   (tid : thread_identifier)
   (cm : casemate_model_state) : casemate_model_state :=
   (* Reset the authorizations for both states *)
-  reset_write_authorizations_aux tid cm.(cm_roots).(pr_s2)
-    (reset_write_authorizations_aux tid cm.(cm_roots).(pr_s1) cm).
+  reset_write_authorizations_aux tid cm.(cms_roots).(cmr_s2)
+    (reset_write_authorizations_aux tid cm.(cms_roots).(cmr_s1) cm).
 
 Definition step_dsb (tid : thread_identifier) (dk : DxB) (cm : casemate_model_state) : casemate_model_result :=
   (* There is enough barrier now to write plain again *)
@@ -796,13 +864,49 @@ Definition is_leaf (kind : pte_rec) : bool :=
   | _ => true
   end.
 
-Definition is_last_level_only (d : TLBI_op_by_addr_data) : bool :=
-  match d.(TOBAD_last_level_only) with
-  | TLBILevel_Any => false
-  | TLBILevel_Last => true
+Definition get_tlbi_asid (td : TLBI_intermediate) : option addr_id_t :=
+  match td.(TI_method) with
+  | TLBI_by_input_addr d => d.(TOBAD_asid)
+  | TLBI_by_addr_space (PA addr_id) => Some (AID addr_id)
+  | _ => None
   end.
 
-Definition should_perform_tlbi (td : TLBI_intermediate) (ptc : pgtable_traverse_context) : option bool :=
+Fixpoint all_children_invalid_iter
+  (idx : u64)
+  (n_children : nat)
+  (table_start : phys_addr_t)
+  (cm : casemate_model_state) : bool :=
+  match n_children with
+  | O => true
+  | S n_children =>
+    let child_addr := table_start pa+ (PA (b8 b* idx)) in
+    match cm !! child_addr with
+    | Some child_loc =>
+      match child_loc.(sl_pte) with
+      | None => false
+      | Some child_pte_desc =>
+        match child_pte_desc.(eed_pte_kind) with
+        | PTER_PTE_KIND_INVALID =>
+          all_children_invalid_iter (idx b+ b1) n_children table_start cm
+        | _ => false
+        end
+      end
+    | None => false
+    end
+  end.
+
+Definition all_children_invalid (pte_desc : entry_exploded_descriptor) (cm : casemate_model_state): bool :=
+  match pte_desc.(eed_pte_kind) with
+  | PTER_PTE_KIND_TABLE table_data =>
+    let table_start := table_data.(next_level_table_addr) in
+    all_children_invalid_iter b0 512 table_start cm
+  | _ => true
+  end.
+
+Definition should_perform_tlbi 
+  (cpu_id : thread_identifier)
+  (td : TLBI_intermediate)
+  (ptc : pgtable_traverse_context) : option bool :=
   match ptc.(ptc_loc) with
   | None => None (* does not happen because we call it in tlbi_visitor in which we test that the location is init *)
   | Some loc =>
@@ -812,32 +916,67 @@ Definition should_perform_tlbi (td : TLBI_intermediate) (ptc : pgtable_traverse_
       match td.(TI_method) with
       | TLBI_by_input_addr d =>
         let tlbi_addr := bv_shiftl_64 (phys_addr_val d.(TOBAD_page)) b12 in
-        let ia_start := pte_desc.(ged_ia_region).(range_start) in
-        let ia_end := ia_start pa+ pte_desc.(ged_ia_region).(range_size) in
-        if (is_leaf pte_desc.(ged_pte_kind)
-                 && (phys_addr_val ia_start b<=? tlbi_addr)
-                 && (tlbi_addr b<? phys_addr_val ia_end)) then
+        let ia_start := pte_desc.(eed_ia_region).(range_start) in
+        let ia_end := ia_start pa+ pte_desc.(eed_ia_region).(range_size) in
+
+        (* If the PTE has valid children, the TLBI by VA is not enough *)
+        if (negb (is_leaf pte_desc.(eed_pte_kind)) && negb (all_children_invalid pte_desc ptc.(ptc_state))) then
           Some false
-        else if ((negb (is_l3 pte_desc.(ged_level))) && is_last_level_only d) then
+
+        (* __should_perform_tlbi_matches_addr *)
+        else if negb ((phys_addr_val ia_start b<=? tlbi_addr)
+                  && (tlbi_addr b<? phys_addr_val ia_end)) then Some false
+        
+        (* __should_perform_tlbi_matches_level *)
+        else if ((negb (is_l3 pte_desc.(eed_level))) && d.(TOBAD_last_level_only)) then
           Some false
+
         else
-          Some true
+          (* __should_perform_tlbi_matches_id *)
+          match td.(TI_regime), pte_desc.(eed_stage) with
+          | TLBI_REGIME_EL10, S2 =>
+            match retrieve_root_for_baddr S2 ptc.(ptc_state).(cms_roots) ptc.(ptc_root) with
+            | Some pte_root =>
+              match get_current_vttbr cpu_id ptc.(ptc_state) with
+              | Some vttbr => Some (bool_decide (pte_root.(r_id) = vttbr.(r_id)))
+              | None => Some true
+              end
+            | None => Some true
+            end
+          | TLBI_REGIME_EL2, S1 =>
+            match retrieve_root_for_baddr S1 ptc.(ptc_state).(cms_roots) ptc.(ptc_root) with
+            | Some pte_root =>
+              match get_tlbi_asid td with
+              | Some asid => Some (bool_decide (pte_root.(r_id) = asid))
+              | None => Some true
+              end
+            | None => Some true
+            end
+          | _, _ => Some true
+          end
       | TLBI_by_addr_space addr_id =>
-        match td.(TI_regime), td.(TI_stage) with
-        (* for VMID *)
-        | Regime_EL10, TLBI_OP_stage2 =>
-            (*pte_root = retrieve_root_for_baddr roots_s2 ptc.(pgtable_traverse_context root)*)
-            (*get_current_vttbr()->id == pte_root->id)*)
-            Some true
-        (* for ASID *)
-        | Regime_EL2, TLBI_OP_stage1 =>
-            (*retrieve_root_for_baddr roots_s1 ptc.(pgtable_traverse_context root)*)
-            (*__get_tlbi_asid(tlbi, &asid)*)
-            (*if asid != pte_root-> id*)
-            Some true
+        match td.(TI_regime), pte_desc.(eed_stage) with
+        | TLBI_REGIME_EL10, S2 =>
+          match retrieve_root_for_baddr S2 ptc.(ptc_state).(cms_roots) ptc.(ptc_root) with
+          | Some pte_root =>
+            match get_current_vttbr cpu_id ptc.(ptc_state) with
+            | Some vttbr => Some (bool_decide (pte_root.(r_id) = vttbr.(r_id)))
+            | None => Some true
+            end
+          | None => Some true
+          end
+        | TLBI_REGIME_EL2, S1 =>
+          match retrieve_root_for_baddr S1 ptc.(ptc_state).(cms_roots) ptc.(ptc_root) with
+          | Some pte_root =>
+            match get_tlbi_asid td with
+            | Some asid => Some (bool_decide (pte_root.(r_id) = asid))
+            | None => Some true
+            end
+          | None => Some true
+          end
         | _, _ => Some true
         end
-      | TLBI_by_addr_all => Some true
+      | TLBI_by_all => Some true
       end
     end
   end.
@@ -845,8 +984,8 @@ Definition should_perform_tlbi (td : TLBI_intermediate) (ptc : pgtable_traverse_
 
 Definition step_pte_on_tlbi_after_dsb (td: TLBI_intermediate) : option LIS :=
   match td.(TI_regime) with
-  | Regime_EL2 => Some LIS_dsb_tlbied
-  | Regime_EL10 =>
+  | TLBI_REGIME_EL2 => Some LIS_dsb_tlbied
+  | TLBI_REGIME_EL10 =>
     match td.(TI_stage) with
     | TLBI_OP_stage1 => Some LIS_dsbed (* no effect*)
     | TLBI_OP_stage2 => Some LIS_dsb_tlbi_ipa
@@ -857,7 +996,7 @@ Definition step_pte_on_tlbi_after_dsb (td: TLBI_intermediate) : option LIS :=
 
 Definition step_pte_on_tlbi_after_tlbi_ipa (td: TLBI_intermediate) : option LIS :=
   match td.(TI_regime) with
-  | Regime_EL10 =>
+  | TLBI_REGIME_EL10 =>
       match td.(TI_stage) with
       | TLBI_OP_stage1 | TLBI_OP_both_stages => Some LIS_dsb_tlbied
       | TLBI_OP_stage2 => Some LIS_dsb_tlbi_ipa_dsb
@@ -875,7 +1014,7 @@ Definition tlbi_visitor
     Merror (CME_uninitialised "tlbi_visitor" ptc.(ptc_addr))
   | Some location =>
     (* Test if there is something to do *)
-    match should_perform_tlbi td ptc with
+    match should_perform_tlbi cpu_id td ptc with
     | None => Merror CME_unimplemented
     | Some b =>
       if b then
@@ -884,7 +1023,7 @@ Definition tlbi_visitor
         | None => Merror (CME_internal_error IET_unexpected_none)
           (* This cannot happen (otherwise, should_perform_tlbi would be false) *)
         | Some exploded_desc =>
-          match exploded_desc.(ged_state) with
+          match exploded_desc.(eed_state) with
           | SPS_STATE_PTE_INVALID_UNCLEAN ai =>
             (* If the CPU that does the transformation is not the one that initiated the invalidation, do nothing *)
             if bool_decide (cpu_id = ai.(ai_invalidator_tid)) then
@@ -908,8 +1047,8 @@ Definition tlbi_visitor
                   end
                 in
                 (* Write the new sub-state in the global automaton *)
-                let new_loc := location <| sl_pte := Some (exploded_desc <|ged_state := SPS_STATE_PTE_INVALID_UNCLEAN (ai <| ai_lis := new_substate|>) |>)|> in
-                let new_mem := ptc.(ptc_state) <| cm_memory := <[location.(sl_phys_addr) := new_loc]> ptc.(ptc_state).(cm_memory)|> in
+                let new_loc := location <| sl_pte := Some (exploded_desc <|eed_state := SPS_STATE_PTE_INVALID_UNCLEAN (ai <| ai_lis := new_substate|>) |>)|> in
+                let new_mem := ptc.(ptc_state) <| cms_memory := <[location.(sl_phys_addr) := new_loc]> ptc.(ptc_state).(cms_memory)|> in
                 log (Mreturn new_mem)
               end
             else
@@ -922,22 +1061,23 @@ Definition tlbi_visitor
     end
   end.
 
-Definition step_tlbi (tid : thread_identifier) (td : TLBI) (cm : casemate_model_state) : casemate_model_result :=
-  match decode_tlbi td with
-  | None => Merror CME_unimplemented
-  | Some decoded_TLBI =>
-    match td.(TLBI_rec).(TLBIRecord_regime) with
-    | Regime_EL2 =>
-      (* traverse all s1 pages*)
-      traverse_si_pgt (Some tid) cm (tlbi_visitor tid decoded_TLBI) S1
-    | Regime_EL10 =>
-      (* traverse s2 pages *)
-      traverse_si_pgt (Some tid) cm (tlbi_visitor tid decoded_TLBI) S2
-    | _ =>
-      (* traverse all page tables and add a warning *)
-      let res := traverse_all_pgt (Some tid) cm (tlbi_visitor tid decoded_TLBI) in
-      res <| cmr_log := Warning_unsupported_TLBI :: res.(cmr_log) |>
-    end
+Definition step_tlbi 
+  (tid : thread_identifier)
+  (td : trans_tlbi_data)
+  (cm : casemate_model_state) :
+  casemate_model_result :=
+  let tlbi := decode_tlbi td in
+  match tlbi.(TI_regime) with
+  | TLBI_REGIME_EL10 =>
+    (* TLBIs that hit host/guest tables *)
+    traverse_pgt (Some tid) cm (tlbi_visitor tid tlbi) S2
+  | TLBI_REGIME_EL2 =>
+    (* TLBIs that hit pKVM's own pagetable *)
+    traverse_pgt (Some tid) cm (tlbi_visitor tid tlbi) S1
+  | _ =>
+    Merror CME_unimplemented
+    (* let res := traverse_all_pgt (Some tid) cm (tlbi_visitor tid tlbi) in
+    res <| cmr_log := Warning_unsupported_TLBI :: res.(cmr_log) |> *)
   end.
 
 (** MSR *)
@@ -948,50 +1088,112 @@ Fixpoint root_exists (root : sm_owner_t) (roots : list cm_root) : bool :=
   | t :: q => (bool_decide (t.(r_baddr) = root)) || (root_exists root q)
   end.
 
-Definition register_root
+Definition try_register_root
   (tid : thread_identifier)
   (addr_id : addr_id_t)
   (cm : casemate_model_state)
-  (root : sm_owner_t)
+  (baddr : sm_owner_t)
   (stage : entry_stage_t) :
   casemate_model_result :=
-  let other_root_list :=
-    match stage with
-    | S1 => pr_s2
-    | S2 => pr_s1
-    end cm.(cm_roots) in
-  (* Check that the root does not already exist in the other root list*)
-  if root_exists root other_root_list then Merror CME_root_already_exists
-  else
-    (* Add the root to the list of roots *)
-    let new_roots :=
-      let new_root := {| r_baddr := root; r_id := addr_id; r_refcount := b0 |} in
-      match stage with
-      | S2 => cm.(cm_roots) <| pr_s2 := new_root :: cm.(cm_roots).(pr_s2) |>
-      | S1 => cm.(cm_roots) <| pr_s1 := new_root :: cm.(cm_roots).(pr_s1) |>
-      end
-    in
-    let new_st := cm <| cm_roots := new_roots |> in
-    (* then mark all its children as PTE *)
-    match root with
-    | Root r => traverse_pgt_from root r pa0 l0 stage (mark_cb tid) new_st
-    end.
+  (* Add the root to the list of roots *)
+  let new_root := {| r_baddr := baddr; r_id := addr_id; r_refcount := 0 |} in
+  let new_roots := insert_cms_root stage new_root cm.(cms_roots) in
+  let new_st := cm <| cms_roots := new_roots |> in
+  (* then mark all its children as PTE *)
+  match baddr with
+  | Root r => traverse_pgt_from baddr r pa0 l0 stage (mark_cb tid) new_st
+  end.
 
-Definition step_msr (tid : thread_identifier) (md : trans_msr_data) (cm : casemate_model_state) : casemate_model_result :=
-  let stage :=
-    match md.(tmd_sysreg) with
-    | SYSREG_TTBR_EL2 => S1
-    | SYSREG_VTTBR => S2
-    end
-  in
-  let root := ttbr_extract_baddr md.(tmd_val) in
+Definition check_ttbr0_el2_asid
+  (md : trans_msr_data)
+  (addr_id : addr_id_t) : bool :=
+  (* TTBR0_EL2 in non-VHE mode has a Res0 ASID *)
+  match md.(tmd_sysreg), addr_id with
+  | SYSREG_TTBR_EL2, AID aid => aid b=? b0
+  | SYSREG_VTTBR, _ => true
+  end.
+
+Definition context_switch
+  (tid : thread_identifier)
+  (addr_id : addr_id_t)
+  (stage : entry_stage_t)
+  (md : trans_msr_data)
+  (cm : casemate_model_state) : 
+  casemate_model_result :=
+  (* decrement refcount on current root (if applicable) *)
+  let assoc_root := current_thread_context_root tid stage cm in
+  let decr_cm := 
+    match assoc_root with
+    | Some root =>
+      let new_assoc_root := {| 
+        r_baddr := root.(r_baddr);
+        r_id := root.(r_id);
+        r_refcount := root.(r_refcount) - 1 |} in
+      let new_cms_roots := update_cms_root_for_baddr stage (root.(r_baddr)) new_assoc_root cm.(cms_roots) in
+      cm <| cms_roots := new_cms_roots |>
+    | None => cm
+    end in
+
+  (* and increment refcount on cone we just switched to *)
+  let assoc_root := retrieve_root_for_id stage decr_cm.(cms_roots) addr_id in
+  match assoc_root with
+  | Some root =>
+    let new_assoc_root := {| 
+      r_baddr := root.(r_baddr);
+      r_id := root.(r_id);
+      r_refcount := root.(r_refcount) + 1 |} in
+    let new_cms_roots := update_cms_root_for_id stage (root.(r_id)) new_assoc_root cm.(cms_roots) in
+    let incr_cm := decr_cm <| cms_roots := new_cms_roots |> in
+    (* make it the curent context *)
+    let final_cm := update_current_thread_context tid stage root.(r_baddr) incr_cm in
+    Mreturn final_cm
+  | None => Merror (CME_internal_error IET_unexpected_none)
+  end.
+
+Definition stage_from_ttbr
+  (sysreg : ghost_sysreg_kind) : entry_stage_t :=
+  match sysreg with
+  | SYSREG_TTBR_EL2 => S1
+  | SYSREG_VTTBR => S2
+  end.
+
+Definition step_msr 
+  (tid : thread_identifier)
+  (md : trans_msr_data)
+  (cm : casemate_model_state) : 
+  casemate_model_result :=
+  let stage := stage_from_ttbr md.(tmd_sysreg) in
+  let baddr := ttbr_extract_baddr md.(tmd_val) in
   let addr_id := ttbr_extract_id md.(tmd_val) in
-  (* The value written to TTRB is a root, it might be new. *)
-  if root_exists root (match stage with | S2 => pr_s2 | S1 => pr_s1 end cm.(cm_roots)) then
-    Mreturn cm (* If it is already known to be a root, do nothing, it has already been registered *)
+
+  (* TTBR0_EL2 in non-VHE mode has a Res0 ASID *)
+  if negb (check_ttbr0_el2_asid md addr_id) then
+    Merror (CME_addr_id_error "TTBR0_EL2 ASID is reserved 0")
   else
-    (* Otherwise, register it *)
-    register_root tid addr_id cm root stage.
+    match retrieve_root_for_baddr stage cm.(cms_roots) baddr with
+    | Some assoc_root =>
+      (* if that root with that id exists already, were just context switching *)
+      if (bool_decide (assoc_root.(r_id) = addr_id)) then
+        context_switch tid addr_id stage md cm
+      else
+        (* see if that root is already associated with a different (VM/AS)ID *)
+        Merror (CME_addr_id_error "root already associated with an (VM/AS)ID")
+    | None =>
+      let res :=
+        match retrieve_root_for_id stage cm.(cms_roots) addr_id with
+        | Some assoc_root =>
+          if negb (bool_decide (assoc_root.(r_baddr) = baddr)) then
+            Merror (CME_addr_id_error "duplicate (VM/AS)ID")
+          else if negb (bool_decide (assoc_root.(r_id) = addr_id)) then
+            Merror (CME_addr_id_error "root already associated with an (VM/AS)ID")
+          else try_register_root tid addr_id cm baddr stage
+        | None => try_register_root tid addr_id cm baddr stage
+        end in
+      match res.(cmr_data) with
+      | Ok _ _ cm => context_switch tid addr_id stage md cm
+      | _ => res
+      end
+    end.
 
 (** Hint *)
 
@@ -1000,7 +1202,7 @@ Definition step_hint_set_root_lock
   (addr : phys_addr_t)
   (cm : casemate_model_state) :
   casemate_model_result :=
-    Mreturn (cm <| cm_lock_addr := insert (phys_addr_val (root_val root)) (phys_addr_val addr) cm.(cm_lock_addr)|>).
+    Mreturn (cm <| cms_lock_addr := insert (phys_addr_val (root_val root)) (phys_addr_val addr) cm.(cms_lock_addr)|>).
 
 Function set_owner_root
   (phys : phys_addr_t)
@@ -1025,12 +1227,12 @@ Function set_owner_root
       let new_pte :=
         match location.(sl_pte) with
         | None => None
-        | Some pte => Some (pte <| ged_owner := root|>) (* actually change the root *)
+        | Some pte => Some (pte <| eed_owner := root|>) (* actually change the root *)
         end
       in
       (* Write the change to the global state *)
       let new_loc := location <| sl_pte := new_pte |> in
-      let new_state := cm <|cm_memory := <[ location.(sl_phys_addr) := new_loc ]> cm.(cm_memory) |> in
+      let new_state := cm <|cms_memory := <[ location.(sl_phys_addr) := new_loc ]> cm.(cms_memory) |> in
       set_owner_root phys root new_state logs (offs - 1)
     end
 .
@@ -1045,7 +1247,7 @@ Definition step_release_cb (ctx : pgtable_traverse_context) : casemate_model_res
     match location.(sl_pte) with
     | None => Merror (CME_not_a_pte "release_cb" ctx.(ptc_addr))
     | Some desc =>
-      match desc.(ged_state) with
+      match desc.(eed_state) with
       | SPS_STATE_PTE_INVALID_UNCLEAN _ =>
           Merror (CME_bbm_violation VT_release_unclean ctx.(ptc_addr))
       | _ => Mreturn ctx.(ptc_state)
@@ -1059,16 +1261,6 @@ Fixpoint remove (x : sm_owner_t) (l : list sm_owner_t) : list sm_owner_t :=
   | nil => nil
   | y :: tl => if bool_decide (x = y) then remove x tl else y::(remove x tl)
   end.
-
-Definition retrieve_root_for_baddr
-  (roots : list cm_root)
-  (root : sm_owner_t) : option cm_root :=
-  find (fun elem => bool_decide (elem.(r_baddr) = root)) roots.
-
-Definition retrieve_root_for_id
-  (roots : list cm_root)
-  (addr_id : addr_id_t) : option cm_root :=
-  find (fun elem => bool_decide (elem.(r_id) = addr_id)) roots.
 
 Fixpoint unregister_root
   (addr : sm_owner_t)
@@ -1093,13 +1285,13 @@ Definition try_unregister_root
     | None => Merror (CME_internal_error IET_unexpected_none)
     | Some pte =>
       let new_roots :=
-        match pte.(ged_stage) with
-        | S2 => cm.(cm_roots) <| pr_s2 := unregister_root addr [] cm.(cm_roots).(pr_s2) |>
-        | S1 => cm.(cm_roots) <| pr_s1 := unregister_root addr [] cm.(cm_roots).(pr_s1) |>
+        match pte.(eed_stage) with
+        | S2 => cm.(cms_roots) <| cmr_s2 := unregister_root addr [] cm.(cms_roots).(cmr_s2) |>
+        | S1 => cm.(cms_roots) <| cmr_s1 := unregister_root addr [] cm.(cms_roots).(cmr_s1) |>
         end
       in
-      let cm := cm <| cm_roots := new_roots |> in
-      traverse_pgt_from_root addr pte.(ged_stage) (unmark_cb cpu) cm
+      let cm := cm <| cms_roots := new_roots |> in
+      traverse_pgt_from_root addr pte.(eed_stage) (unmark_cb cpu) cm
     end
   end.
 
@@ -1116,10 +1308,10 @@ Definition step_release_table
     | Some desc =>
       let new_st := traverse_pgt_from
         addr
-        (root_val desc.(ged_owner))
-        desc.(ged_ia_region).(range_start)
-        desc.(ged_level)
-        desc.(ged_stage)
+        (root_val desc.(eed_owner))
+        desc.(eed_ia_region).(range_start)
+        desc.(eed_level)
+        desc.(eed_stage)
         step_release_cb
         cm in
       Mupdate_state (try_unregister_root (addr) cpu) new_st
@@ -1138,9 +1330,9 @@ Definition step_hint_set_pte_thread_owner
     match location.(sl_pte) with
     | None => Merror (CME_not_a_pte "set_pte_thread_owner"%string phys)
     | Some _ =>
-      let thread_owner := Thread_identifier (to_nat (phys_addr_val (root_val val))) in
-      Mreturn (cm <| cm_memory :=
-        (<[ location.(sl_phys_addr) := location <| sl_thread_owner := Some thread_owner |> ]> cm.(cm_memory))
+      let thread_owner := TID (phys_addr_val (root_val val)) in
+      Mreturn (cm <| cms_memory :=
+        (<[ location.(sl_phys_addr) := location <| sl_thread_owner := Some thread_owner |> ]> cm.(cms_memory))
       |> )
     end
   end
@@ -1174,10 +1366,10 @@ Definition step_lock
   (hd : trans_lock_data)
   (cm : casemate_model_state) :
   casemate_model_result :=
-  match lookup (phys_addr_val hd.(tld_addr)) cm.(cm_lock_state) with
+  match lookup (phys_addr_val hd.(tld_addr)) cm.(cms_lock_state) with
   | None => (* give the lock write_authorization to write the page-table *)
     let lock_state := {| ls_tid := cpu; ls_write_authorization := WA_AUTHORIZED |} in
-    Mreturn (cm <| cm_lock_state := insert (phys_addr_val hd.(tld_addr)) lock_state cm.(cm_lock_state) |>)
+    Mreturn (cm <| cms_lock_state := insert (phys_addr_val hd.(tld_addr)) lock_state cm.(cms_lock_state) |>)
   | Some {| ls_tid := thread; ls_write_authorization := _ |} => Merror (CME_double_lock_acquire cpu thread)
   end
 .
@@ -1187,10 +1379,10 @@ Definition step_unlock
   (hd : trans_lock_data)
   (cm : casemate_model_state) : 
   casemate_model_result :=
-  match lookup (phys_addr_val hd.(tld_addr)) cm.(cm_lock_state) with
+  match lookup (phys_addr_val hd.(tld_addr)) cm.(cms_lock_state) with
   | Some {| ls_tid := thread; ls_write_authorization := _ |} =>
     if bool_decide (thread = cpu) then
-      Mreturn (cm <| cm_lock_state := delete (phys_addr_val hd.(tld_addr)) cm.(cm_lock_state) |>)
+      Mreturn (cm <| cms_lock_state := delete (phys_addr_val hd.(tld_addr)) cm.(cms_lock_state) |>)
     else
       Merror (CME_double_lock_acquire cpu thread)
   | None => Merror (CME_double_lock_acquire cpu cpu)
